code/rsapss/Hacl.Bignum.fst
@@ -16,14 +16,17 @@ let bn_add aLen a bLen b res =
 let bn_sub aLen a bLen b res =
   Hacl.Bignum.Addition.bn_sub aLen a bLen b res
 
-let bn_add_mod_n len n a b res =
+let bn_reduce_once len n c0 res =
   push_frame ();
   let tmp = create len (u64 0) in
-  let c0 = bn_add_eq_len len a b res in
   let c1 = bn_sub_eq_len len res n tmp in
   let c = c0 -. c1 in
   map2T len res (Hacl.Spec.Bignum.Definitions.mask_select c) res tmp;
   pop_frame()
+
+let bn_add_mod_n len n a b res =
+  let c0 = bn_add_eq_len len a b res in
+  bn_reduce_once len n c0 res
 
 let bn_mul aLen a bLen b res =
   Hacl.Bignum.Multiplication.bn_mul aLen a bLen b res
