code/rsapss/Hacl.Spec.Bignum.Exponentiation.fst
@@ -16,18 +16,17 @@ module M = Hacl.Spec.Montgomery.Lemmas
 #reset-options "--z3rlimit 50 --fuel 0 --ifuel 0"
 
 val bn_mod_exp_f:
-    #nLen:size_nat
-  -> #rLen:size_nat{rLen = nLen + 1 /\ rLen + rLen <= max_size_t}
+    #nLen:size_pos{nLen + nLen <= max_size_t}
   -> n:lbignum nLen
   -> mu:uint64
   -> bBits:size_pos
   -> bLen:size_nat{bLen == blocks bBits 64}
   -> b:lbignum bLen
   -> i:nat{i < bBits}
-  -> aM_accM: tuple2 (lbignum rLen) (lbignum rLen) ->
-  tuple2 (lbignum rLen) (lbignum rLen)
+  -> aM_accM: tuple2 (lbignum nLen) (lbignum nLen) ->
+  tuple2 (lbignum nLen) (lbignum nLen)
 
-let bn_mod_exp_f #nLen #rLen n mu bBits bLen b i (aM, accM) =
+let bn_mod_exp_f #nLen n mu bBits bLen b i (aM, accM) =
   let accM = if (bn_is_bit_set #bLen b i) then mont_mul n mu aM accM else accM in // acc = (acc * a) % n
   let aM = mont_sqr n mu aM in // a = (a * a) % n
   (aM, accM)
@@ -35,7 +34,7 @@ let bn_mod_exp_f #nLen #rLen n mu bBits bLen b i (aM, accM) =
 
 val bn_mod_exp_mont:
     modBits:size_pos
-  -> nLen:size_pos{128 * (nLen + 1) <= max_size_t}
+  -> nLen:size_pos{128 * nLen <= max_size_t}
   -> n:lbignum nLen{nLen == blocks modBits 64}
   -> a:lbignum nLen
   -> acc:lbignum nLen
@@ -44,16 +43,14 @@ val bn_mod_exp_mont:
   lbignum nLen
 
 let bn_mod_exp_mont modBits nLen n a acc bBits b =
-  let rLen = nLen + 1 in
   let bLen = blocks bBits 64 in
   let mu = mod_inv_u64 n.[0] in
 
   let r2 = precomp_r2_mod_n #nLen modBits n in
   let aM = to_mont n mu r2 a in
   let accM = to_mont n mu r2 acc in
-  let (aM, accM) = repeati bBits (bn_mod_exp_f #nLen #rLen n mu bBits bLen b) (aM, accM) in
-  let res = from_mont n mu accM in
-  bn_sub_mask n res
+  let (aM, accM) = repeati bBits (bn_mod_exp_f #nLen n mu bBits bLen b) (aM, accM) in
+  from_mont n mu accM
 
 let bn_mod_exp modBits nLen n a bBits b =
   let acc = bn_from_uint nLen (u64 1) in
@@ -62,88 +59,83 @@ let bn_mod_exp modBits nLen n a bBits b =
 
 
 val bn_mod_exp_f_lemma:
-    #nLen:size_nat
-  -> #rLen:size_nat{rLen = nLen + 1 /\ rLen + rLen <= max_size_t}
+    #nLen:size_nat{nLen + nLen <= max_size_t}
   -> n:lbignum nLen
   -> mu:uint64
   -> bBits:size_pos
   -> bLen:size_nat{bLen == blocks bBits 64}
   -> b:lbignum bLen
   -> i:nat{i < bBits}
-  -> aM_accM0: tuple2 (lbignum rLen) (lbignum rLen) -> Lemma
+  -> aM_accM0: tuple2 (lbignum nLen) (lbignum nLen) -> Lemma
   (requires
    (let (aM0, accM0) = aM_accM0 in
     (1 + (bn_v n % pow2 64) * v mu) % pow2 64 == 0 /\
     bn_v n % 2 = 1 /\ 1 < bn_v n /\ bn_v n < pow2 (64 * nLen) /\
     0 < bn_v b /\ bn_v b < pow2 bBits /\
-    bn_v aM0 < 2 * bn_v n /\ bn_v accM0 < 2 * bn_v n))
+    bn_v aM0 < bn_v n /\ bn_v accM0 < bn_v n))
   (ensures
    (let (aM0, accM0) = aM_accM0 in
-    let (aM1, accM1) = bn_mod_exp_f #nLen #rLen n mu bBits bLen b i aM_accM0 in
-    let (aM2, accM2) = BL.mod_exp_f_ll rLen (bn_v n) (v mu) bBits (bn_v b) i (bn_v aM0, bn_v accM0) in
+    let (aM1, accM1) = bn_mod_exp_f #nLen n mu bBits bLen b i aM_accM0 in
+    let (aM2, accM2) = BL.mod_exp_f_ll nLen (bn_v n) (v mu) bBits (bn_v b) i (bn_v aM0, bn_v accM0) in
     bn_v aM1 == aM2 /\ bn_v accM1 == accM2 /\
-    bn_v aM1 < 2 * bn_v n /\ bn_v accM1 < 2 * bn_v n))
+    bn_v aM1 < bn_v n /\ bn_v accM1 < bn_v n))
 
-let bn_mod_exp_f_lemma #nLen #rLen n mu bBits bLen b i (aM0, accM0) =
-  let (aM1, accM1) = bn_mod_exp_f #nLen #rLen n mu bBits bLen b i (aM0, accM0) in
-  let (aM2, accM2) = BL.mod_exp_f_ll rLen (bn_v n) (v mu) bBits (bn_v b) i (bn_v aM0, bn_v accM0) in
-  mont_sqr_lemma #nLen #rLen n mu aM0;
+let bn_mod_exp_f_lemma #nLen n mu bBits bLen b i (aM0, accM0) =
+  let (aM1, accM1) = bn_mod_exp_f #nLen n mu bBits bLen b i (aM0, accM0) in
+  let (aM2, accM2) = BL.mod_exp_f_ll nLen (bn_v n) (v mu) bBits (bn_v b) i (bn_v aM0, bn_v accM0) in
+  mont_sqr_lemma #nLen n mu aM0;
   assert (bn_v aM1 == aM2);
   bn_is_bit_set_lemma #bLen b i;
-  if (bn_v b / pow2 i % 2 = 1) then mont_mul_lemma #nLen #rLen n mu aM0 accM0;
-  assert (bn_v accM1 == accM2);
-  let d, k = M.eea_pow2_odd (64 * rLen) (bn_v n) in
-  M.mont_preconditions nLen (bn_v n) (v mu);
-  BL.mod_exp_mont_ll_lemma_fits_loop_step rLen (bn_v n) d (v mu) bBits (bn_v b) i (bn_v aM0) (bn_v accM0)
+  if (bn_v b / pow2 i % 2 = 1) then mont_mul_lemma #nLen n mu aM0 accM0;
+  assert (bn_v accM1 == accM2)
 
 
 val bn_mod_exp_mont_loop_lemma:
-    #nLen:size_nat
-  -> #rLen:size_nat{rLen = nLen + 1 /\ rLen + rLen <= max_size_t}
+    #nLen:size_nat{nLen + nLen <= max_size_t}
   -> n:lbignum nLen
   -> mu:uint64
   -> bBits:size_pos
   -> bLen:size_nat{bLen == blocks bBits 64}
   -> b:lbignum bLen
   -> i:size_nat{i <= bBits}
-  -> aM_accM0: tuple2 (lbignum rLen) (lbignum rLen) -> Lemma
+  -> aM_accM0: tuple2 (lbignum nLen) (lbignum nLen) -> Lemma
   (requires
    (let (aM0, accM0) = aM_accM0 in
     (1 + (bn_v n % pow2 64) * v mu) % pow2 64 == 0 /\
     bn_v n % 2 = 1 /\ 1 < bn_v n /\ bn_v n < pow2 (64 * nLen) /\
     0 < bn_v b /\ bn_v b < pow2 bBits /\
-    bn_v aM0 < 2 * bn_v n /\ bn_v accM0 < 2 * bn_v n))
+    bn_v aM0 < bn_v n /\ bn_v accM0 < bn_v n))
   (ensures
    (let (aM0, accM0) = aM_accM0 in
-    let (aM1, accM1) = repeati i (bn_mod_exp_f #nLen #rLen n mu bBits bLen b) (aM0, accM0) in
-    let (aM2, accM2) = repeati i (BL.mod_exp_f_ll rLen (bn_v n) (v mu) bBits (bn_v b)) (bn_v aM0, bn_v accM0) in
+    let (aM1, accM1) = repeati i (bn_mod_exp_f #nLen n mu bBits bLen b) (aM0, accM0) in
+    let (aM2, accM2) = repeati i (BL.mod_exp_f_ll nLen (bn_v n) (v mu) bBits (bn_v b)) (bn_v aM0, bn_v accM0) in
     bn_v aM1 == aM2 /\ bn_v accM1 == accM2 /\
-    bn_v aM1 < 2 * bn_v n /\ bn_v accM1 < 2 * bn_v n))
+    bn_v aM1 < bn_v n /\ bn_v accM1 < bn_v n))
 
-let rec bn_mod_exp_mont_loop_lemma #nLen #rLen n mu bBits bLen b i (aM0, accM0) =
-  let (aM1, accM1) = repeati i (bn_mod_exp_f #nLen #rLen n mu bBits bLen b) (aM0, accM0) in
-  let (aM2, accM2) = repeati i (BL.mod_exp_f_ll rLen (bn_v n) (v mu) bBits (bn_v b)) (bn_v aM0, bn_v accM0) in
+let rec bn_mod_exp_mont_loop_lemma #nLen n mu bBits bLen b i (aM0, accM0) =
+  let (aM1, accM1) = repeati i (bn_mod_exp_f #nLen n mu bBits bLen b) (aM0, accM0) in
+  let (aM2, accM2) = repeati i (BL.mod_exp_f_ll nLen (bn_v n) (v mu) bBits (bn_v b)) (bn_v aM0, bn_v accM0) in
 
   if i = 0 then begin
-    eq_repeati0 i (bn_mod_exp_f #nLen #rLen n mu bBits bLen b) (aM0, accM0);
-    eq_repeati0 i (BL.mod_exp_f_ll rLen (bn_v n) (v mu) bBits (bn_v b)) (bn_v aM0, bn_v accM0);
+    eq_repeati0 i (bn_mod_exp_f #nLen n mu bBits bLen b) (aM0, accM0);
+    eq_repeati0 i (BL.mod_exp_f_ll nLen (bn_v n) (v mu) bBits (bn_v b)) (bn_v aM0, bn_v accM0);
     () end
   else begin
-    unfold_repeati i (bn_mod_exp_f #nLen #rLen n mu bBits bLen b) (aM0, accM0) (i - 1);
-    unfold_repeati i (BL.mod_exp_f_ll rLen (bn_v n) (v mu) bBits (bn_v b)) (bn_v aM0, bn_v accM0) (i - 1);
-    let (aM3, accM3) = repeati (i - 1) (bn_mod_exp_f #nLen #rLen n mu bBits bLen b) (aM0, accM0) in
-    let (aM4, accM4) = repeati (i - 1) (BL.mod_exp_f_ll rLen (bn_v n) (v mu) bBits (bn_v b)) (bn_v aM0, bn_v accM0) in
-    assert ((aM1, accM1) == bn_mod_exp_f #nLen #rLen n mu bBits bLen b (i - 1) (aM3, accM3));
-    assert ((aM2, accM2) == BL.mod_exp_f_ll rLen (bn_v n) (v mu) bBits (bn_v b) (i - 1) (aM4, accM4));
-    bn_mod_exp_mont_loop_lemma #nLen #rLen n mu bBits bLen b (i - 1) (aM0, accM0);
+    unfold_repeati i (bn_mod_exp_f #nLen n mu bBits bLen b) (aM0, accM0) (i - 1);
+    unfold_repeati i (BL.mod_exp_f_ll nLen (bn_v n) (v mu) bBits (bn_v b)) (bn_v aM0, bn_v accM0) (i - 1);
+    let (aM3, accM3) = repeati (i - 1) (bn_mod_exp_f #nLen n mu bBits bLen b) (aM0, accM0) in
+    let (aM4, accM4) = repeati (i - 1) (BL.mod_exp_f_ll nLen (bn_v n) (v mu) bBits (bn_v b)) (bn_v aM0, bn_v accM0) in
+    assert ((aM1, accM1) == bn_mod_exp_f #nLen n mu bBits bLen b (i - 1) (aM3, accM3));
+    assert ((aM2, accM2) == BL.mod_exp_f_ll nLen (bn_v n) (v mu) bBits (bn_v b) (i - 1) (aM4, accM4));
+    bn_mod_exp_mont_loop_lemma #nLen n mu bBits bLen b (i - 1) (aM0, accM0);
     assert (bn_v aM3 == aM4 /\ bn_v accM3 == accM4);
-    bn_mod_exp_f_lemma #nLen #rLen n mu bBits bLen b (i - 1) (aM3, accM3);
+    bn_mod_exp_f_lemma #nLen n mu bBits bLen b (i - 1) (aM3, accM3);
     () end
 
 
 val bn_mod_exp_mont_lemma_aux:
     modBits:size_pos
-  -> nLen:size_pos{nLen = (blocks modBits 64) /\ 128 * (nLen + 1) <= max_size_t}
+  -> nLen:size_pos{nLen = (blocks modBits 64) /\ 128 * nLen <= max_size_t}
   -> n:lbignum nLen
   -> a:lbignum nLen
   -> bBits:size_pos
@@ -154,11 +146,10 @@ val bn_mod_exp_mont_lemma_aux:
   (ensures
    (let mu = mod_inv_u64 n.[0] in
     let res1 = bn_mod_exp modBits nLen n a bBits b in
-    let res2 = BL.mod_exp_mont_ll (nLen + 1) (bn_v n) (v mu) (bn_v a) bBits (bn_v b) in
+    let res2 = BL.mod_exp_mont_ll nLen (bn_v n) (v mu) (bn_v a) bBits (bn_v b) in
     bn_v res1 == res2 /\ bn_v res1 < bn_v n))
 
 let bn_mod_exp_mont_lemma_aux modBits nLen n a bBits b =
-  let rLen = nLen + 1 in
   let bLen = blocks bBits 64 in
 
   let acc = bn_from_uint nLen (u64 1) in
@@ -174,26 +165,24 @@ let bn_mod_exp_mont_lemma_aux modBits nLen n a bBits b =
 
   let r2 = precomp_r2_mod_n modBits n in
   precomp_r2_mod_n_lemma modBits n;
-  let aM0 = to_mont #nLen #rLen n mu r2 a in
-  to_mont_lemma #nLen #rLen n mu r2 a;
+  let aM0 = to_mont #nLen n mu r2 a in
+  to_mont_lemma #nLen n mu r2 a;
 
-  let accM0 = to_mont #nLen #rLen n mu r2 acc in
-  to_mont_lemma #nLen #rLen n mu r2 acc;
+  let accM0 = to_mont #nLen n mu r2 acc in
+  to_mont_lemma #nLen n mu r2 acc;
 
-  let (aM1, accM1) = repeati bBits (bn_mod_exp_f #nLen #rLen n mu bBits bLen b) (aM0, accM0) in
-  bn_mod_exp_mont_loop_lemma #nLen #rLen n mu bBits bLen b bBits (aM0, accM0);
+  let (aM1, accM1) = repeati bBits (bn_mod_exp_f #nLen n mu bBits bLen b) (aM0, accM0) in
+  bn_mod_exp_mont_loop_lemma #nLen n mu bBits bLen b bBits (aM0, accM0);
 
   let res = from_mont n mu accM1 in
-  from_mont_lemma #nLen #rLen n mu accM1;
-  assert (bn_v res <= bn_v n);
-  bn_sub_mask_lemma n res
+  from_mont_lemma #nLen n mu accM1
 
 
 let bn_mod_exp_lemma modBits nLen n a bBits b =
   let mu = mod_inv_u64 n.[0] in
   let r2 = precomp_r2_mod_n modBits n in
   let res1 = bn_mod_exp modBits nLen n a bBits b in
-  let res2 = BL.mod_exp_mont_ll (nLen + 1) (bn_v n) (v mu) (bn_v a) bBits (bn_v b) in
+  let res2 = BL.mod_exp_mont_ll nLen (bn_v n) (v mu) (bn_v a) bBits (bn_v b) in
   bn_mod_exp_mont_lemma_aux modBits nLen n a bBits b;
   assert (bn_v res1 == res2 /\ bn_v res1 < bn_v n);
 
@@ -204,6 +193,6 @@ let bn_mod_exp_lemma modBits nLen n a bBits b =
   mod_inv_u64_lemma n.[0];
   assert ((1 + (bn_v n % pow2 64) * v mu) % pow2 64 == 0);
 
-  let d, k = M.eea_pow2_odd (64 * (nLen + 1)) (bn_v n) in
+  let d, k = M.eea_pow2_odd (64 * nLen) (bn_v n) in
   M.mont_preconditions nLen (bn_v n) (v mu);
-  BL.mod_exp_mont_ll_lemma (nLen + 1) (bn_v n) d (v mu) (bn_v a) bBits (bn_v b)
+  BL.mod_exp_mont_ll_lemma nLen (bn_v n) d (v mu) (bn_v a) bBits (bn_v b)
