code/rsapss/Hacl.Spec.Bignum.Montgomery.fst
@@ -6,10 +6,9 @@ open Lib.IntTypes
 open Lib.Sequence
 open Lib.LoopCombinators
 
+open Hacl.Spec.Bignum.Base
 open Hacl.Spec.Bignum.Definitions
 open Hacl.Spec.Bignum
-
-friend Hacl.Spec.Bignum // TODO: avoid using a friend mechanism for this module
 
 #reset-options "--z3rlimit 100 --fuel 0 --ifuel 0"
 
@@ -120,6 +119,8 @@ let mod_inv_u64_inv_step_even n0 i ub0 vb0 =
     };
   assert (2 * (ub * 2 * v alpha - vb * v beta) == pow2 (64 - i + 1))
 
+
+#push-options "--z3rlimit 150"
 val mod_inv_u64_inv_step_odd: n0:uint64 -> i:pos{i <= 64} -> ub0:uint64 -> vb0:uint64 -> Lemma
   (requires
    (let alpha = u64 1 <<. 63ul in let beta = n0 in
@@ -163,7 +164,7 @@ let mod_inv_u64_inv_step_odd n0 i ub0 vb0 =
     pow2 (64 - i + 1);
   };
   assert (2 * (ub * 2 * v alpha - vb * v beta) == pow2 (64 - i + 1))
-
+#pop-options
 
 val mod_inv_u64_inv_step: n0:uint64 -> i:pos{i <= 64} -> ub0:uint64 -> vb0:uint64 -> Lemma
   (requires
@@ -276,9 +277,9 @@ let rec bn_mul_by_pow2 len n b k =
 let precomp_r2_mod_n #nLen modBits n =
   let c = create nLen (u64 0) in
   let c0 = bn_bit_set c (modBits - 1) in // c0 == pow2 (modBits - 1)
-  // pow2 (128 * (nLen + 1)) / pow2 (modBits - 1) == pow2 (128 * nLen + 129 - modBits)
+  // pow2 (128 * nLen) / pow2 (modBits - 1) == pow2 (128 * nLen + 1 - modBits)
 
-  repeati (128 * nLen + 129 - modBits) (bn_lshift1_mod_n n) c0
+  repeati (128 * nLen + 1 - modBits) (bn_lshift1_mod_n n) c0
 
 
 let precomp_r2_mod_n_lemma #nLen modBits n =
@@ -287,377 +288,293 @@ let precomp_r2_mod_n_lemma #nLen modBits n =
   bn_eval_zeroes nLen nLen;
   bn_bit_set_lemma c (modBits - 1);
   assert (bn_v c0 == pow2 (modBits - 1));
-  let res = repeati (128 * nLen + 129 - modBits) (bn_lshift1_mod_n n) c0 in
-  bn_mul_by_pow2 nLen n c0 (128 * nLen + 129 - modBits);
-  assert (bn_v res == pow2 (128 * nLen + 129 - modBits) * pow2 (modBits - 1) % bn_v n);
-  Math.Lemmas.pow2_plus (128 * nLen + 129 - modBits) (modBits - 1);
-  assert (bn_v res == pow2 (128 * nLen + 128) % bn_v n)
+  let res = repeati (128 * nLen + 1 - modBits) (bn_lshift1_mod_n n) c0 in
+  bn_mul_by_pow2 nLen n c0 (128 * nLen + 1 - modBits);
+  assert (bn_v res == pow2 (128 * nLen + 1 - modBits) * pow2 (modBits - 1) % bn_v n);
+  Math.Lemmas.pow2_plus (128 * nLen + 1 - modBits) (modBits - 1);
+  assert (bn_v res == pow2 (128 * nLen) % bn_v n)
 
 ///
 ///  Low-level specification of Montgomery arithmetic
 ///
 
 val mont_reduction_f:
-    #nLen:size_nat
-  -> #rLen:size_nat{rLen = nLen + 1 /\ rLen + rLen <= max_size_t}
+    #nLen:size_nat{nLen + nLen <= max_size_t}
   -> n:lbignum nLen
   -> mu:uint64
-  -> j:size_nat{j < rLen}
-  -> acc:lbignum (rLen + rLen) ->
-  lbignum (rLen + rLen)
+  -> j:size_nat{j < nLen}
+  -> tuple2 carry (lbignum (nLen + nLen)) ->
+  tuple2 carry (lbignum (nLen + nLen))
 
-let mont_reduction_f #nLen #rLen n mu j acc =
+let mont_reduction_f #nLen n mu j (c0, acc) =
   let qj = mu *. acc.[j] in
-  let c, res1 = bn_mul1_lshift_add #nLen #(rLen + rLen) n qj j acc in
+  let c1, res1 = bn_mul1_lshift_add #nLen #(nLen + nLen) n qj j acc in
+  let c2, r = addcarry_u64 c0 c1 res1.[nLen + j] in
+  let res = res1.[nLen + j] <- r in
+  c2, res
 
-  let res2 = slice res1 (j + nLen) (rLen + rLen) in
-  let _, res3 = bn_add res2 (create 1 c) in
-  update_sub res1 (j + nLen) (rLen + rLen - j - nLen) res3
+let mont_reduction_t (#nLen:size_nat{nLen + nLen <= max_size_t}) (j:size_nat{j <= nLen}) =
+  tuple2 carry (lbignum (nLen + nLen))
 
+let mont_reduction #nLen n mu c =
+  let (c0, c) = repeat_gen nLen mont_reduction_t (mont_reduction_f #nLen n mu) (u64 0, c) in
+  let res = bn_rshift c nLen in
+  bn_reduce_once n c0 res
 
-let mont_reduction #nLen #rLen n mu c =
-  let c = repeati rLen (mont_reduction_f #nLen #rLen n mu) c in
-  bn_rshift c rLen
-
-
-let to_mont #nLen #rLen n mu r2 a =
+let to_mont #nLen n mu r2 a =
   let c = bn_mul a r2 in // c = a * r2
-  let tmp = create (rLen + rLen) (u64 0) in
-  let tmp = update_sub tmp 0 (nLen + nLen) c in
-  mont_reduction #nLen #rLen n mu tmp // aM = c % n
+  mont_reduction #nLen n mu c // aM = c % n
 
+let from_mont #nLen n mu aM =
+  let tmp = create (nLen + nLen) (u64 0) in
+  let tmp = update_sub tmp 0 nLen aM in
+  mont_reduction #nLen n mu tmp
 
-let from_mont #nLen #rLen n mu aM =
-  let tmp = create (rLen + rLen) (u64 0) in
-  let tmp = update_sub tmp 0 rLen aM in
-  let a' = mont_reduction #nLen #rLen n mu tmp in
-  sub a' 0 nLen
-
-
-let mont_mul #nLen #rLen n mu aM bM =
+let mont_mul #nLen n mu aM bM =
   let c = bn_mul aM bM in // c = aM * bM
   mont_reduction n mu c // resM = c % n
 
-let mont_sqr #nLen #rLen n mu aM =
+let mont_sqr #nLen n mu aM =
   let c = bn_sqr aM in // c = aM * aM
   mont_reduction n mu c // resM = c % n
 
 
+val eq_slice: #a:Type0 -> #len:size_nat -> b1:lseq a len -> b2:lseq a len -> i:nat -> j:nat{i <= j /\ j <= len} -> Lemma
+  (requires slice b1 i len == slice b2 i len)
+  (ensures  slice b1 j len == slice b2 j len)
 
-val mont_reduction_f_carry:
-    #nLen:size_nat
-  -> #rLen:size_nat{rLen = nLen + 1 /\ rLen + rLen <= max_size_t}
+let eq_slice #a #len b1 b2 i j =
+  let aux (k:nat{k < len - j}) : Lemma (index (slice b1 j len) k == index (slice b2 j len) k) =
+    Seq.lemma_index_slice b1 i len (k + j - i);
+    Seq.lemma_index_slice b2 i len (k + j - i);
+    () in
+
+  Classical.forall_intro aux;
+  eq_intro (slice b1 j len) (slice b2 j len)
+
+
+val mont_reduction_f_eval_lemma:
+    #nLen:size_nat{nLen + nLen <= max_size_t}
   -> n:lbignum nLen
   -> mu:uint64
-  -> j:size_nat{j < rLen}
-  -> acc:lbignum (rLen + rLen) ->
-  uint64 & lbignum (rLen + rLen)
+  -> j:size_nat{j < nLen}
+  -> cres0:tuple2 carry (lbignum (nLen + nLen)) ->
+  Lemma (
+    let (c0, res0) = cres0 in
+    let (c2, res) = mont_reduction_f #nLen n mu j (c0, res0) in
+    let qj = mu *. res0.[j] in
+    eval_ (nLen + nLen) res (nLen + j + 1) + v c2 * pow2 (64 * (nLen + j + 1)) ==
+    eval_ (nLen + nLen) res0 (nLen + j + 1) + bn_v n * v qj * pow2 (64 * j) + v c0 * pow2 (64 * (nLen + j)) /\
+    slice res (nLen + j + 1) (nLen + nLen) == slice res0 (nLen + j + 1) (nLen + nLen))
 
-let mont_reduction_f_carry #nLen #rLen n mu j acc =
-  let qj = mu *. acc.[j] in
-  let c, res1 = bn_mul1_lshift_add #nLen #(rLen + rLen) n qj j acc in
+let mont_reduction_f_eval_lemma #nLen n mu j (c0, res0) =
+  let p = pow2 (64 * (nLen + j)) in
+  let resLen = nLen + nLen in
+  let qj = mu *. res0.[j] in
+  let c1, res1 = bn_mul1_lshift_add #nLen #resLen n qj j res0 in
+  bn_mul1_lshift_add_lemma #nLen #resLen n qj j res0;
+  assert (v c1 * p + eval_ resLen res1 (nLen + j) == eval_ resLen res0 (nLen + j) + bn_v n * v qj * pow2 (64 * j));
 
-  let res2 = slice res1 (j + nLen) (rLen + rLen) in
-  let c1, res3 = bn_add res2 (create 1 c) in
-  c1, update_sub res1 (j + nLen) (rLen + rLen - j - nLen) res3
+  let c2, r = addcarry_u64 c0 c1 res1.[nLen + j] in
+  assert (v r + v c2 * pow2 64 == v c0 + v c1 + v res1.[nLen + j]);
+  let res = res1.[nLen + j] <- r in
+  bn_eval_extensionality_j res res1 (nLen + j);
+  assert (eval_ resLen res (nLen + j) == eval_ resLen res1 (nLen + j));
+  bn_eval_unfold_i res (nLen + j + 1);
+  assert (eval_ resLen res (nLen + j + 1) == eval_ resLen res1 (nLen + j) + p * v res.[nLen + j]);
 
-
-val mont_reduction_f_lemma_bound:
-    #nLen:size_nat
-  -> #rLen:size_nat{rLen = nLen + 1 /\ rLen + rLen <= max_size_t}
-  -> n:lbignum nLen
-  -> qj:uint64
-  -> c:lbignum (rLen + rLen)
-  -> j:size_nat{j < rLen}
-  -> acc:lbignum (rLen + rLen) -> Lemma
-  (requires
-    0 < bn_v n /\ bn_v n < pow2 (64 * nLen) /\
-    bn_v c < 4 * bn_v n * bn_v n /\
-    bn_v acc <= bn_v c + (pow2 (64 * j) - 1) * bn_v n)
-  (ensures
-    bn_v acc + bn_v n * v qj * pow2 (64 * j) <= bn_v c + (pow2 (64 * (j + 1)) - 1) * bn_v n /\
-    bn_v acc + bn_v n * v qj * pow2 (64 * j) < pow2 (128 * rLen))
-
-let mont_reduction_f_lemma_bound #nLen #rLen n qj c j acc =
-  M.mont_reduction_lemma_step_bound_aux rLen (bn_v n) (v qj) (j + 1) (bn_v c) (bn_v acc);
-  calc (<) {
-    bn_v c + (pow2 (64 * (j + 1)) - 1) * bn_v n;
-    (<) { Math.Lemmas.pow2_le_compat (64 * rLen) (64 * (j + 1)) }
-    bn_v c + pow2 (64 * rLen) * bn_v n;
-    (<) { }
-    4 * bn_v n * bn_v n + pow2 (64 * rLen) * bn_v n;
-    (<) { M.mont_preconditions_rLen nLen (bn_v n);
-      Math.Lemmas.lemma_mult_lt_right (bn_v n) (4 * bn_v n) (pow2 (64 * (nLen + 1))) }
-    pow2 (64 * rLen) * bn_v n + pow2 (64 * rLen) * bn_v n;
-    (==) { Math.Lemmas.pow2_plus 1 (64 * rLen) }
-    pow2 (1 + 64 * rLen) * bn_v n;
-    (<) { Math.Lemmas.lemma_mult_lt_left (pow2 (1 + 64 * rLen)) (bn_v n) (pow2 (64 * nLen)) }
-    pow2 (1 + 64 * rLen) * pow2 (64 * nLen);
-    (==) { Math.Lemmas.pow2_plus (1 + 64 * rLen) (64 * nLen) }
-    pow2 (1 + 64 * rLen + 64 * nLen);
-    (<) { Math.Lemmas.pow2_lt_compat (64 * rLen + 64 * rLen) (1 + 64 * rLen + 64 * nLen) }
-    pow2 (128 * rLen);
-  };
-  assert (bn_v c + (pow2 (64 * (j + 1)) - 1) * bn_v n < pow2 (128 * rLen))
-
-
-val mont_reduction_f_lemma_aux:
-  nLen:nat -> resLen:nat{resLen == nLen + nLen + 2} -> a:nat -> b:nat -> c:nat -> j:nat{j <= nLen} -> Lemma
-  (pow2 (64 * (nLen + j)) * (a + b - c * pow2 (64 * (resLen - j - nLen))) + pow2 (64 * resLen) * c ==
-   pow2 (64 * (nLen + j)) * a + pow2 (64 * (nLen + j)) * b)
-let mont_reduction_f_lemma_aux nLen resLen a b c j =
   calc (==) {
-    pow2 (64 * (nLen + j)) * (a + b - c * pow2 (64 * (resLen - j - nLen)));
-    (==) { Math.Lemmas.distributivity_sub_right (pow2 (64 * (nLen + j))) (a + b) (c * pow2 (64 * (resLen - j - nLen))) }
-    pow2 (64 * (nLen + j)) * (a + b) - pow2 (64 * (nLen + j)) * c * pow2 (64 * (resLen - j - nLen));
-    (==) { Math.Lemmas.distributivity_add_right (pow2 (64 * (nLen + j))) a b }
-    pow2 (64 * (nLen + j)) * a + pow2 (64 * (nLen + j)) * b - pow2 (64 * (nLen + j)) * c * pow2 (64 * (resLen - j - nLen));
-    (==) { Math.Lemmas.paren_mul_right (pow2 (64 * (nLen + j))) (pow2 (64 * (resLen - j - nLen))) c }
-    pow2 (64 * (nLen + j)) * a + pow2 (64 * (nLen + j)) * b - pow2 (64 * (nLen + j)) * pow2 (64 * (resLen - j - nLen)) * c;
-    (==) { Math.Lemmas.pow2_plus (64 * (nLen + j)) (64 * (resLen - nLen - j)) }
-    pow2 (64 * (nLen + j)) * a + pow2 (64 * (nLen + j)) * b - pow2 (64 * resLen) * c;
+    eval_ resLen res1 (nLen + j) + p * v res.[nLen + j];
+    (==) { }
+    eval_ resLen res0 (nLen + j) + bn_v n * v qj * pow2 (64 * j) - v c1 * p + p * (v c0 + v c1 + v res1.[nLen + j] - v c2 * pow2 64);
+    (==) { Math.Lemmas.distributivity_add_right p (v c1) (v c0 + v res1.[nLen + j] - v c2 * pow2 64) }
+    eval_ resLen res0 (nLen + j) + bn_v n * v qj * pow2 (64 * j) + p * (v c0 + v res1.[nLen + j] - v c2 * pow2 64);
+    (==) { Math.Lemmas.distributivity_add_right p (v res1.[nLen + j]) (v c0 - v c2 * pow2 64) }
+    eval_ resLen res0 (nLen + j) + bn_v n * v qj * pow2 (64 * j) + p * v res1.[nLen + j] + p * (v c0 - v c2 * pow2 64);
+    (==) { Seq.lemma_index_slice res1 (nLen + j) resLen 0 }
+    eval_ resLen res0 (nLen + j) + bn_v n * v qj * pow2 (64 * j) + p * v res0.[nLen + j] + p * (v c0 - v c2 * pow2 64);
+    (==) { bn_eval_unfold_i res0 (nLen + j + 1) }
+    eval_ resLen res0 (nLen + j + 1) + bn_v n * v qj * pow2 (64 * j) + p * (v c0 - v c2 * pow2 64);
+    (==) { Math.Lemmas.distributivity_sub_right p (v c0) (v c2 * pow2 64) }
+    eval_ resLen res0 (nLen + j + 1) + bn_v n * v qj * pow2 (64 * j) + p * v c0 - p * v c2 * pow2 64;
+    (==) { Math.Lemmas.pow2_plus (64 * (nLen + j)) 64 }
+    eval_ resLen res0 (nLen + j + 1) + bn_v n * v qj * pow2 (64 * j) + p * v c0 - pow2 (64 * (nLen + j + 1)) * v c2;
   };
-  assert (pow2 (64 * (nLen + j)) * (a + b - c * pow2 (64 * (resLen - j - nLen))) ==
-    pow2 (64 * (nLen + j)) * a + pow2 (64 * (nLen + j)) * b - pow2 (64 * resLen) * c)
 
-
-val mont_reduction_f_carry_lemma:
-    #nLen:size_nat
-  -> #rLen:size_nat{rLen = nLen + 1 /\ rLen + rLen <= max_size_t}
-  -> n:lbignum nLen
-  -> mu:uint64
-  -> c:lbignum (rLen + rLen)
-  -> j:size_nat{j < rLen}
-  -> acc:lbignum (rLen + rLen) -> Lemma
-   (let c1, res = mont_reduction_f_carry #nLen #rLen n mu j acc in
-    let qj = mu *. acc.[j] in
-    bn_v res + pow2 (128 * rLen) * v c1 == bn_v acc + bn_v n * v qj * pow2 (64 * j))
-
-let mont_reduction_f_carry_lemma #nLen #rLen n mu c j acc =
-  let resLen = rLen + rLen in
-  let qj = mu *. acc.[j] in
-  let c, res1 = bn_mul1_lshift_add #nLen #resLen n qj j acc in
-  bn_mul1_lshift_add_lemma #nLen #(rLen+rLen) n qj j acc;
-  assert (v c * pow2 (64 * (nLen + j)) + eval_ resLen res1 (nLen + j) == eval_ resLen acc (nLen + j) + bn_v n * v qj * pow2 (64 * j));
-
-  let res2 = slice res1 (j + nLen) resLen in
-  let acc2 = slice acc (j + nLen) resLen in
-  assert (res1 == update_sub acc j nLen (snd (Hacl.Spec.Bignum.Multiplication.bn_mul1_add_in_place #nLen n qj (sub acc j nLen))));
-  eq_intro res2 acc2;
-  assert (res2 == acc2);
-
-  let c1, res3 = bn_add res2 (create 1 c) in
-  bn_add_lemma res2 (create 1 c);
-  bn_eval_create1 c;
-  assert (v c1 * pow2 (64 * (resLen - j - nLen)) + bn_v res3 == bn_v acc2 + v c);
-
-  let res4 = update_sub res1 (j + nLen) (resLen - j - nLen) res3 in
-  calc (==) {
-    bn_v res4 + pow2 (64 * resLen) * v c1;
-    (==) { bn_eval_split_i res4 (j + nLen) }
-    bn_v (slice res4 0 (j + nLen)) + pow2 (64 * (j + nLen)) * bn_v (slice res4 (j + nLen) resLen) + pow2 (64 * resLen) * v c1;
-    (==) { }
-    bn_v (slice res4 0 (j + nLen)) + pow2 (64 * (j + nLen)) * bn_v res3 + pow2 (64 * resLen) * v c1;
-    (==) { eq_intro (sub res4 0 (j + nLen)) (sub res1 0 (j + nLen)) }
-    bn_v (slice res1 0 (j + nLen)) + pow2 (64 * (j + nLen)) * bn_v res3 + pow2 (64 * resLen) * v c1;
-    (==) { }
-    bn_v (slice res1 0 (nLen + j)) + pow2 (64 * (nLen + j)) * (bn_v acc2 + v c - v c1 * pow2 (64 * (resLen - j - nLen))) + pow2 (64 * resLen) * v c1;
-    (==) { bn_eval_extensionality_j res1 (slice res1 0 (nLen + j)) (nLen + j) }
-    eval_ resLen res1 (nLen + j) + pow2 (64 * (nLen + j)) * (bn_v acc2 + v c - v c1 * pow2 (64 * (resLen - j - nLen))) + pow2 (64 * resLen) * v c1;
-    (==) { }
-    eval_ resLen acc (nLen + j) + bn_v n * v qj * pow2 (64 * j) - v c * pow2 (64 * (nLen + j)) +
-      pow2 (64 * (nLen + j)) * (bn_v acc2 + v c - v c1 * pow2 (64 * (resLen - j - nLen))) + pow2 (64 * resLen) * v c1;
-    (==) { mont_reduction_f_lemma_aux nLen resLen (bn_v acc2) (v c) (v c1) j }
-    eval_ resLen acc (nLen + j) + bn_v n * v qj * pow2 (64 * j) + pow2 (64 * (nLen + j)) * bn_v acc2;
-    (==) { bn_eval_extensionality_j acc (slice acc 0 (nLen + j)) (nLen + j) }
-    bn_v (slice acc 0 (nLen + j)) + bn_v n * v qj * pow2 (64 * j) + pow2 (64 * (nLen + j)) * bn_v acc2;
-    (==) { }
-    bn_v (slice acc 0 (nLen + j)) + pow2 (64 * (nLen + j)) * bn_v acc2 + bn_v n * v qj * pow2 (64 * j);
-    (==) { bn_eval_split_i acc (nLen + j) }
-    bn_v acc + bn_v n * v qj * pow2 (64 * j);
-  };
-  assert (bn_v res4 + pow2 (64 * resLen) * v c1 == bn_v acc + bn_v n * v qj * pow2 (64 * j))
-
-
-val mont_reduction_f_carry_drop_lemma:
-    #nLen:size_nat
-  -> #rLen:size_nat{rLen = nLen + 1 /\ rLen + rLen <= max_size_t}
-  -> n:lbignum nLen
-  -> mu:uint64
-  -> c:lbignum (rLen + rLen)
-  -> j:size_nat{j < rLen}
-  -> acc:lbignum (rLen + rLen) -> Lemma
-  (requires
-    0 < bn_v n /\ bn_v n < pow2 (64 * nLen) /\
-    bn_v c < 4 * bn_v n * bn_v n /\
-    bn_v acc <= bn_v c + (pow2 (64 * j) - 1) * bn_v n)
-  (ensures
-   (let res = mont_reduction_f #nLen #rLen n mu j acc in
-    bn_v res == bn_v acc + bn_v n * (v mu * v acc.[j] % pow2 64) * pow2 (64 * j) /\
-    bn_v res <= bn_v c + (pow2 (64 * (j + 1)) - 1) * bn_v n))
-
-let mont_reduction_f_carry_drop_lemma #nLen #rLen n mu c j acc =
-  let c1, res = mont_reduction_f_carry #nLen #rLen n mu j acc in
-  let qj = mu *. acc.[j] in
-  mont_reduction_f_carry_lemma #nLen #rLen n mu c j acc;
-  assert (bn_v res + pow2 (128 * rLen) * v c1 == bn_v acc + bn_v n * v qj * pow2 (64 * j));
-  mont_reduction_f_lemma_bound #nLen #rLen n qj c j acc;
-  assert (bn_v acc + bn_v n * v qj * pow2 (64 * j) < pow2 (128 * rLen));
-  assert (v c1 = 0)
+  eq_slice res0 res1 (nLen + j) (nLen + j + 1);
+  eq_intro (slice res (nLen + j + 1) (nLen + nLen)) (slice res0 (nLen + j + 1) (nLen + nLen))
 
 
 val mont_reduction_f_lemma:
-    #nLen:size_nat
-  -> #rLen:size_nat{rLen = nLen + 1 /\ rLen + rLen <= max_size_t}
+    #nLen:size_nat{nLen + nLen <= max_size_t}
   -> n:lbignum nLen
   -> mu:uint64
-  -> c:lbignum (rLen + rLen)
-  -> j:size_nat{j < rLen}
-  -> acc:lbignum (rLen + rLen) -> Lemma
-  (requires
-    0 < bn_v n /\ bn_v n < pow2 (64 * nLen) /\
-    bn_v c < 4 * bn_v n * bn_v n /\
-    bn_v acc <= bn_v c + (pow2 (64 * j) - 1) * bn_v n)
-  (ensures
-   (let res = mont_reduction_f #nLen #rLen n mu j acc in
-    bn_v res == M.smont_reduction_f rLen (bn_v n) (v mu) j (bn_v acc) /\
-    bn_v res <= bn_v c + (pow2 (64 * (j + 1)) - 1) * bn_v n))
+  -> j:size_nat{j < nLen}
+  -> cres0:tuple2 carry (lbignum (nLen + nLen)) ->
+  Lemma (
+    let (c0, res0) = cres0 in
+    let (c2, res) = mont_reduction_f #nLen n mu j (c0, res0) in
+    let qj = mu *. res0.[j] in
+    bn_v res + v c2 * pow2 (64 * (nLen + j + 1)) ==
+    bn_v res0 + bn_v n * v qj * pow2 (64 * j) + v c0 * pow2 (64 * (nLen + j)))
 
-let mont_reduction_f_lemma #nLen #rLen n mu c j acc =
-  let res = mont_reduction_f #nLen #rLen n mu j acc in
-  mont_reduction_f_carry_drop_lemma #nLen #rLen n mu c j acc;
-  bn_eval_index acc j;
-  assert (v acc.[j] == bn_v acc / pow2 (64 * j) % pow2 64)
+let mont_reduction_f_lemma #nLen n mu j (c0, res0) =
+  let (c2, res) = mont_reduction_f #nLen n mu j (c0, res0) in
+  mont_reduction_f_eval_lemma #nLen n mu j (c0, res0);
+  bn_eval_split_i res (nLen + j + 1);
+  bn_eval_split_i res0 (nLen + j + 1);
+  bn_eval_extensionality_j res (slice res 0 (nLen + j + 1)) (nLen + j + 1);
+  bn_eval_extensionality_j res0 (slice res0 0 (nLen + j + 1)) (nLen + j + 1)
+
+
+val mont_reduction_loop_step_lemma:
+    #nLen:size_nat{nLen + nLen <= max_size_t}
+  -> n:lbignum nLen{0 < bn_v n}
+  -> mu:uint64
+  -> j:size_nat{j < nLen}
+  -> c1:carry
+  -> res1:lbignum (nLen + nLen)
+  -> resM1:nat -> Lemma
+  (requires
+    v c1 * pow2 (64 * (nLen + j)) + bn_v res1 == resM1)
+  (ensures
+    (let (c2, res) = mont_reduction_f #nLen n mu j (c1, res1) in
+     let resM = M.mont_reduction_f nLen (bn_v n) (v mu) j resM1 in
+     v c2 * pow2 (64 * (nLen + j + 1)) + bn_v res == resM))
+
+let mont_reduction_loop_step_lemma #nLen n mu j c1 res1 resM1 =
+  let (c2, res) = mont_reduction_f #nLen n mu j (c1, res1) in
+  let resM = M.mont_reduction_f nLen (bn_v n) (v mu) j resM1 in
+  mont_reduction_f_lemma #nLen n mu j (c1, res1);
+  let qj = mu *. res1.[j] in
+  assert (bn_v res + v c2 * pow2 (64 * (nLen + j + 1)) ==
+    bn_v res1 + bn_v n * v qj * pow2 (64 * j) + v c1 * pow2 (64 * (nLen + j)));
+  bn_eval_index res1 j;
+  assert (v res1.[j] == bn_v res1 / pow2 (64 * j) % pow2 64);
+  assert (v qj == v mu * v res1.[j] % pow2 64);
+  assert (bn_v res + v c2 * pow2 (64 * (nLen + j + 1)) == resM1 + bn_v n * v qj * pow2 (64 * j));
+  let cjM = resM1 / pow2 (64 * j) % pow2 64 in
+  let qjM = v mu * cjM % pow2 64 in
+  assert (resM == resM1 + bn_v n * qjM * pow2 (64 * j));
+
+  calc (==) {
+    (v c1 * pow2 (64 * (nLen + j)) + bn_v res1) / pow2 (64 * j) % pow2 64;
+    (==) { Math.Lemmas.pow2_plus (64 * nLen) (64 * j) }
+    (v c1 * pow2 (64 * nLen) * pow2 (64 * j) + bn_v res1) / pow2 (64 * j) % pow2 64;
+    (==) { Math.Lemmas.division_addition_lemma (bn_v res1) (pow2 (64 * j)) (v c1 * pow2 (64 * nLen)) }
+    (v c1 * pow2 (64 * nLen) + bn_v res1 / pow2 (64 * j)) % pow2 64;
+    (==) { Math.Lemmas.pow2_plus (64 * (nLen - 1)) 64 }
+    (v c1 * pow2 (64 * (nLen - 1)) * pow2 64 + bn_v res1 / pow2 (64 * j)) % pow2 64;
+    (==) { Math.Lemmas.modulo_addition_lemma (bn_v res1 / pow2 (64 * j)) (pow2 64) (v c1 * pow2 (64 * (nLen - 1))) }
+    (bn_v res1 / pow2 (64 * j)) % pow2 64;
+    }
 
 
 val mont_reduction_loop_lemma:
-    #nLen:size_nat
-  -> #rLen:size_nat{rLen = nLen + 1 /\ rLen + rLen <= max_size_t}
-  -> n:lbignum nLen
+    #nLen:size_nat{nLen + nLen <= max_size_t}
+  -> n:lbignum nLen{0 < bn_v n}
   -> mu:uint64
-  -> c:lbignum (rLen + rLen)
-  -> j:size_nat{j <= rLen} -> Lemma
-  (requires
-    0 < bn_v n /\ bn_v n < pow2 (64 * nLen) /\
-    bn_v c < 4 * bn_v n * bn_v n)
-  (ensures
-   (let res = repeati j (mont_reduction_f #nLen #rLen n mu) c in
-    bn_v res == repeati j (M.smont_reduction_f rLen (bn_v n) (v mu)) (bn_v c) /\
-    bn_v res <= bn_v c + (pow2 (64 * j) - 1) * bn_v n))
+  -> j:size_nat{j <= nLen}
+  -> res0:lbignum (nLen + nLen) ->
+  Lemma (
+    let (c2, res) = repeat_gen j mont_reduction_t (mont_reduction_f #nLen n mu) (u64 0, res0) in
+    let resM = repeati j (M.mont_reduction_f nLen (bn_v n) (v mu)) (bn_v res0) in
+    v c2 * pow2 (64 * (nLen + j)) + bn_v res == resM)
 
-let rec mont_reduction_loop_lemma #nLen #rLen n mu c j =
-  let res1 = repeati j (mont_reduction_f #nLen #rLen n mu) c in
-  let res2 = repeati j (M.smont_reduction_f rLen (bn_v n) (v mu)) (bn_v c) in
+let rec mont_reduction_loop_lemma #nLen n mu j res0 =
+  let (c2, res) = repeat_gen j mont_reduction_t (mont_reduction_f #nLen n mu) (u64 0, res0) in
+  let resM = repeati j (M.mont_reduction_f nLen (bn_v n) (v mu)) (bn_v res0) in
+
   if j = 0 then begin
-    eq_repeati0 j (mont_reduction_f #nLen #rLen n mu) c;
-    eq_repeati0 j (M.smont_reduction_f rLen (bn_v n) (v mu)) (bn_v c) end
+    eq_repeati0 j (M.mont_reduction_f nLen (bn_v n) (v mu)) (bn_v res0);
+    eq_repeat_gen0 j mont_reduction_t (mont_reduction_f #nLen n mu) (u64 0, res0);
+    () end
   else begin
-    unfold_repeati j (mont_reduction_f #nLen #rLen n mu) c (j - 1);
-    unfold_repeati j (M.smont_reduction_f rLen (bn_v n) (v mu)) (bn_v c) (j - 1);
-    let res3 = repeati (j - 1) (mont_reduction_f #nLen #rLen n mu) c in
-    let res4 = repeati (j - 1) (M.smont_reduction_f rLen (bn_v n) (v mu)) (bn_v c) in
-    mont_reduction_loop_lemma #nLen #rLen n mu c (j - 1);
-    assert (bn_v res3 == res4);
-    assert (res1 == mont_reduction_f #nLen #rLen n mu (j - 1) res3);
-    assert (res2 == M.smont_reduction_f rLen (bn_v n) (v mu) (j - 1) res4);
-    assert (bn_v res3 <= bn_v c + (pow2 (64 * (j - 1)) - 1) * bn_v n);
-    mont_reduction_f_lemma #nLen #rLen n mu c (j - 1) res3;
-    assert (bn_v res1 == res2);
+    let (c1, res1) = repeat_gen (j - 1) mont_reduction_t (mont_reduction_f #nLen n mu) (u64 0, res0) in
+    let resM1 = repeati (j - 1) (M.mont_reduction_f nLen (bn_v n) (v mu)) (bn_v res0) in
+    unfold_repeat_gen j mont_reduction_t (mont_reduction_f #nLen n mu) (u64 0, res0) (j - 1);
+    assert ((c2, res) == mont_reduction_f #nLen n mu (j - 1) (c1, res1));
+    unfold_repeati j (M.mont_reduction_f nLen (bn_v n) (v mu)) (bn_v res0) (j - 1);
+    assert (resM == M.mont_reduction_f nLen (bn_v n) (v mu) (j - 1) resM1);
+    mont_reduction_loop_lemma #nLen n mu (j - 1) res0;
+    assert (v c1 * pow2 (64 * (nLen + j - 1)) + bn_v res1 == resM1);
+    mont_reduction_loop_step_lemma #nLen n mu (j - 1) c1 res1 resM1;
     () end
 
 
-let mont_reduction_lemma #nLen #rLen n mu c =
-  let res1 = repeati rLen (mont_reduction_f #nLen #rLen n mu) c in
-  mont_reduction_loop_lemma #nLen #rLen n mu c rLen;
-  bn_rshift_lemma res1 rLen;
-  assert (bn_v (mont_reduction #nLen #rLen n mu c) == M.mont_reduction rLen (bn_v n) (v mu) (bn_v c));
-  let d, k = M.eea_pow2_odd (64 * rLen) (bn_v n) in
+let mont_reduction_lemma #nLen n mu res0 =
+  let resLen = nLen + nLen in
+  let (c0, res1) = repeat_gen nLen mont_reduction_t (mont_reduction_f #nLen n mu) (u64 0, res0) in
+  let resM : nat = repeati nLen (M.mont_reduction_f nLen (bn_v n) (v mu)) (bn_v res0) in
+  mont_reduction_loop_lemma #nLen n mu nLen res0;
+  assert (v c0 * pow2 (64 * resLen) + bn_v res1 == resM);
+  let res2 = bn_rshift res1 nLen in
+  bn_rshift_lemma res1 nLen;
+  assert (bn_v res2 == bn_v res1 / pow2 (64 * nLen));
+
+  calc (==) {
+    (v c0 * pow2 (64 * resLen) + bn_v res1) / pow2 (64 * nLen);
+    (==) { Math.Lemmas.pow2_plus (64 * nLen) (64 * nLen) }
+    (v c0 * pow2 (64 * nLen) * pow2 (64 * nLen) + bn_v res1) / pow2 (64 * nLen);
+    (==) { Math.Lemmas.division_addition_lemma (bn_v res1) (pow2 (64 * nLen)) (v c0 * pow2 (64 * nLen)) }
+    v c0 * pow2 (64 * nLen) + bn_v res1 / pow2 (64 * nLen);
+    (==) { }
+    v c0 * pow2 (64 * nLen) + bn_v res2;
+    };
+
+  let d, k = M.eea_pow2_odd (64 * nLen) (bn_v n) in
   M.mont_preconditions nLen (bn_v n) (v mu);
-  M.mont_mult_lemma_fits rLen (bn_v n) d (v mu) (bn_v c)
+  M.mont_mult_lemma_fits_aux nLen (bn_v n) d (v mu) (bn_v res0);
+  assert (resM / pow2 (64 * nLen) < 2 * bn_v n);
+
+  let res3 = bn_reduce_once n c0 res2 in
+  bn_reduce_once_lemma n c0 res2;
+  assert (bn_v res3 == (v c0 * pow2 (64 * nLen) + bn_v res2) % bn_v n);
+
+  let resM1 = resM / pow2 (64 * nLen) in
+  let resM2 = if resM1 < bn_v n then resM1 else resM1 - bn_v n in
+  Math.Lemmas.lemma_mod_sub resM1 (bn_v n) 1;
+  assert (resM2 % bn_v n == resM1 % bn_v n);
+  M.mont_mult_lemma_fits nLen (bn_v n) d (v mu) (bn_v res0);
+  Math.Lemmas.small_mod resM2 (bn_v n);
+  assert (resM2 == resM1 % bn_v n)
 
 
-val lemma_mult_lt: a:nat -> b:nat -> c:nat -> d:nat -> Lemma
-  (requires a < b /\ c < d)
-  (ensures a * c < b * d)
-let lemma_mult_lt a b c d = ()
-
-
-let to_mont_lemma #nLen #rLen n mu r2 a =
+let to_mont_lemma #nLen n mu r2 a =
   let c = bn_mul a r2 in // c = a * r2
   bn_mul_lemma a r2;
-  lemma_mult_lt (bn_v a) (bn_v n) (bn_v r2) (bn_v n);
+  Math.Lemmas.lemma_mult_lt_sqr (bn_v a) (bn_v r2) (bn_v n);
   assert (bn_v c < bn_v n * bn_v n);
 
-  let tmp = create (rLen + rLen) (u64 0) in
-  let tmp = update_sub tmp 0 (nLen + nLen) c in
-  bn_eval_update_sub (nLen + nLen) c (rLen + rLen);
-  assert (bn_v c == bn_v tmp);
-
-  let aM = mont_reduction #nLen #rLen n mu tmp in // aM = c % n
-  mont_reduction_lemma #nLen #rLen n mu tmp;
-  assert (bn_v aM == M.mont_reduction rLen (bn_v n) (v mu) (bn_v tmp));
-
-  let d, k = M.eea_pow2_odd (64 * rLen) (bn_v n) in
-  M.mont_preconditions nLen (bn_v n) (v mu);
-  M.to_mont_lemma_fits rLen (bn_v n) d (v mu) (bn_v a)
+  let aM = mont_reduction #nLen n mu c in // aM = c % n
+  mont_reduction_lemma #nLen n mu c;
+  assert (bn_v aM == M.mont_reduction nLen (bn_v n) (v mu) (bn_v c))
 
 
-val lemma_top_is_zero:
-    #nLen:size_nat
-  -> #rLen:size_nat{rLen = nLen + 1 /\ rLen + rLen <= max_size_t}
-  -> n:lbignum nLen
-  -> a:lbignum rLen -> Lemma
-  (requires bn_v a <= bn_v n)
-  (ensures  bn_v a == eval_ rLen a nLen)
-
-let lemma_top_is_zero #nLen #rLen n a =
-  bn_eval_split_i a nLen;
-  assert (bn_v a == bn_v (slice a 0 nLen) + pow2 (64 * nLen) * bn_v (slice a nLen rLen));
-  bn_eval_bound n nLen;
-  assert (bn_v a < pow2 (64 * nLen));
-  bn_eval_bound (slice a 0 nLen) nLen;
-  assert (bn_v (slice a 0 nLen) < pow2 (64 * nLen));
-  assert (bn_v a == bn_v (slice a 0 nLen));
-  bn_eval_extensionality_j (slice a 0 nLen) a nLen
-
-
-let from_mont_lemma #nLen #rLen n mu aM =
-  let tmp = create (rLen + rLen) (u64 0) in
-  let tmp = update_sub tmp 0 rLen aM in
-  bn_eval_update_sub rLen aM (rLen + rLen);
+let from_mont_lemma #nLen n mu aM =
+  let tmp = create (nLen + nLen) (u64 0) in
+  let tmp = update_sub tmp 0 nLen aM in
+  bn_eval_update_sub nLen aM (nLen + nLen);
   assert (bn_v tmp == bn_v aM);
 
-  let a' = mont_reduction #nLen #rLen n mu tmp in
+  let a = mont_reduction #nLen n mu tmp in
   mont_reduction_lemma n mu tmp;
-  assert (bn_v a' == M.mont_reduction rLen (bn_v n) (v mu) (bn_v tmp));
-
-  let d, k = M.eea_pow2_odd (64 * rLen) (bn_v n) in
-  M.mont_preconditions nLen (bn_v n) (v mu);
-  M.from_mont_lemma_fits rLen (bn_v n) d (v mu) (bn_v aM);
-  assert (bn_v a' <= bn_v n);
-
-  let res = sub a' 0 nLen in
-  bn_eval_extensionality_j a' res nLen;
-  assert (eval_ nLen res nLen == eval_ rLen a' nLen);
-  assert (bn_v res == eval_ rLen a' nLen);
-  lemma_top_is_zero #nLen #rLen n a';
-  assert (bn_v a' == eval_ rLen a' nLen);
-  assert (bn_v res == M.mont_reduction rLen (bn_v n) (v mu) (bn_v tmp))
+  assert (bn_v a == M.mont_reduction nLen (bn_v n) (v mu) (bn_v tmp))
 
 
-let mont_mul_lemma #nLen #rLen n mu aM bM =
+let mont_mul_lemma #nLen n mu aM bM =
   let c = bn_mul aM bM in
   bn_mul_lemma aM bM;
   assert (bn_v c == bn_v aM * bn_v bM);
-  Math.Lemmas.lemma_mult_lt_sqr (bn_v aM) (bn_v bM) (2 * bn_v n);
-  assert (bn_v c < 4 * bn_v n * bn_v n);
-  mont_reduction_lemma #nLen #rLen n mu c
+  Math.Lemmas.lemma_mult_lt_sqr (bn_v aM) (bn_v bM) (bn_v n);
+  assert (bn_v c < bn_v n * bn_v n);
+  mont_reduction_lemma #nLen n mu c
 
 
-let mont_sqr_lemma #nLen #rLen n mu aM =
+let mont_sqr_lemma #nLen n mu aM =
   let c = bn_sqr aM in
   bn_sqr_lemma aM;
   assert (bn_v c == bn_v aM * bn_v aM);
-  Math.Lemmas.lemma_mult_lt_sqr (bn_v aM) (bn_v aM) (2 * bn_v n);
-  assert (bn_v c < 4 * bn_v n * bn_v n);
-  mont_reduction_lemma #nLen #rLen n mu c
+  Math.Lemmas.lemma_mult_lt_sqr (bn_v aM) (bn_v aM) (bn_v n);
+  assert (bn_v c < bn_v n * bn_v n);
+  mont_reduction_lemma #nLen n mu c
