code/rsapss/Hacl.Spec.Montgomery.Lemmas.fst
@@ -159,39 +159,52 @@ let mont_preconditions_n0 n mu =
   };
   assert ((1 + n * mu) % pow2 64 == 0)
 
+val mont_preconditions:
+  nLen:nat -> n:pos{1 < n /\ n < pow2 (64 * nLen)} -> mu:nat -> Lemma
+  (requires n % 2 = 1 /\ (1 + (n % pow2 64) * mu) % pow2 64 == 0)
+  (ensures
+    (let r = pow2 (64 * nLen) in
+     let d, _ = eea_pow2_odd (64 * nLen) n in
+     r * d % n == 1 /\ n < r /\ (1 + n * mu) % pow2 64 == 0))
+
+let mont_preconditions nLen n mu =
+  mont_preconditions_d nLen n;
+  mont_preconditions_n0 n mu
+
 ///
 ///  High-level specification of Montgomery arithmetic
 ///
 
-val smont_reduction_f: rLen:nat -> n:pos -> mu:nat -> i:nat{i < rLen} -> c:nat -> nat
-let smont_reduction_f rLen n mu i c =
+val mont_reduction_f: rLen:nat -> n:pos -> mu:nat -> i:nat{i < rLen} -> c:nat -> nat
+let mont_reduction_f rLen n mu i c =
   let c_i = c / pow2 (64 * i) % pow2 64 in
   let q_i = mu * c_i % pow2 64 in
   let res = c + n * q_i * pow2 (64 * i) in
   res
 
-val mont_reduction: rLen:nat -> n:pos -> mu:nat -> c:nat -> res:nat
+val mont_reduction: rLen:nat -> n:pos -> mu:nat -> c:nat -> nat
 let mont_reduction rLen n mu c =
-  let res = repeati rLen (smont_reduction_f rLen n mu) c in
-  res / pow2 (64 * rLen)
+  let res = repeati rLen (mont_reduction_f rLen n mu) c in
+  let res = res / pow2 (64 * rLen) in
+  if res < n then res else res - n
 
-val to_mont: rLen:nat -> n:pos -> mu:nat -> a:nat -> aM:nat
+val to_mont: rLen:nat -> n:pos -> mu:nat -> a:nat -> nat
 let to_mont rLen n mu a =
   let r2 = pow2 (128 * rLen) % n in
   let c = a * r2 in
   mont_reduction rLen n mu c
 
-val from_mont: rLen:nat -> n:pos -> mu:nat -> aM:nat -> a:nat
+val from_mont: rLen:nat -> n:pos -> mu:nat -> aM:nat -> nat
 let from_mont rLen n mu aM = mont_reduction rLen n mu aM
 
-val mont_mul: rLen:nat -> n:pos -> mu:nat -> a:nat -> b:nat -> res:nat
+val mont_mul: rLen:nat -> n:pos -> mu:nat -> a:nat -> b:nat -> nat
 let mont_mul rLen n mu a b =
   let c = a * b in
   mont_reduction rLen n mu c
 
 
 ///
-///  Lemma (mont_reduction rLen n mu c % n == c * d % n)
+///  Lemma (mont_reduction rLen n mu c == c * d % n)
 ///
 
 
@@ -201,36 +214,39 @@ val mont_reduction_lemma_step_bound_aux:
   (ensures  res0 + n * q_i * pow2 (64 * (i - 1)) <= c + (pow2 (64 * i) - 1) * n)
 
 let mont_reduction_lemma_step_bound_aux rLen n q_i i c res0 =
+  let b = pow2 (64 * i) in
+  let b1 = pow2 (64 * (i - 1)) in
+
   calc (<=) {
-    res0 + n * q_i * pow2 (64 * (i - 1));
-    (<=) { Math.Lemmas.lemma_mult_le_right (pow2 (64 * (i - 1))) q_i (pow2 64 - 1) }
-    res0 + n * (pow2 64 - 1) * pow2 (64 * (i - 1));
-    (==) { Math.Lemmas.paren_mul_right n (pow2 64 - 1) (pow2 (64 * (i - 1))) }
-    res0 + n * ((pow2 64 - 1) * pow2 (64 * (i - 1)));
-    (==) { Math.Lemmas.distributivity_sub_left (pow2 64) 1 (pow2 (64 * (i - 1))) }
-    res0 + n * (pow2 64 * pow2 (64 * (i - 1)) - pow2 (64 * (i - 1)));
+    res0 + n * q_i * b1;
+    (<=) { Math.Lemmas.lemma_mult_le_right b1 q_i (pow2 64 - 1) }
+    res0 + n * (pow2 64 - 1) * b1;
+    (==) { Math.Lemmas.paren_mul_right n (pow2 64 - 1) b1 }
+    res0 + n * ((pow2 64 - 1) * b1);
+    (==) { Math.Lemmas.distributivity_sub_left (pow2 64) 1 b1 }
+    res0 + n * (pow2 64 * b1 - b1);
     (==) { Math.Lemmas.pow2_plus 64 (64 * (i - 1)) }
-    res0 + n * (pow2 (64 * i) - pow2 (64 * (i - 1)));
-    (==) { Math.Lemmas.distributivity_sub_right n (pow2 (64 * i)) (pow2 (64 * (i - 1))) }
-    res0 + n * pow2 (64 * i) - n * pow2 (64 * (i - 1));
+    res0 + n * (b - b1);
+    (==) { Math.Lemmas.distributivity_sub_right n b b1 }
+    res0 + n * b - n * b1;
     (<=) { }
-    c + (pow2 (64 * (i - 1)) - 1) * n + n * pow2 (64 * i) - n * pow2 (64 * (i - 1));
-    (==) { Math.Lemmas.distributivity_sub_left (pow2 (64 * (i - 1))) 1 n }
-    c + pow2 (64 * (i - 1)) * n - n + n * pow2 (64 * i) - n * pow2 (64 * (i - 1));
+    c + (b1 - 1) * n + n * b - n * b1;
+    (==) { Math.Lemmas.distributivity_sub_left b1 1 n }
+    c + b1 * n - n + n * b - n * b1;
     (==) { }
-    c - n + pow2 (64 * i) * n;
-    (==) { Math.Lemmas.distributivity_sub_left (pow2 (64 * i)) 1 n }
-    c + (pow2 (64 * i) - 1) * n;
+    c - n + b * n;
+    (==) { Math.Lemmas.distributivity_sub_left b 1 n }
+    c + (b - 1) * n;
   }
 
 
 val mont_reduction_lemma_step_bound:
   rLen:nat -> n:pos -> mu:nat -> i:pos{i <= rLen} -> c:nat -> res0:nat -> Lemma
   (requires res0 <= c + (pow2 (64 * (i - 1)) - 1) * n)
-  (ensures  smont_reduction_f rLen n mu (i - 1) res0 <= c + (pow2 (64 * i) - 1) * n)
+  (ensures  mont_reduction_f rLen n mu (i - 1) res0 <= c + (pow2 (64 * i) - 1) * n)
 
 let mont_reduction_lemma_step_bound rLen n mu i c res0 =
-  let res = smont_reduction_f rLen n mu (i - 1) res0 in
+  let res = mont_reduction_f rLen n mu (i - 1) res0 in
   let c_i = res0 / pow2 (64 * (i - 1)) % pow2 64 in
   let q_i = mu * c_i % pow2 64 in
   assert (res == res0 + n * q_i * pow2 (64 * (i - 1)));
@@ -241,52 +257,55 @@ let mont_reduction_lemma_step_bound rLen n mu i c res0 =
 val mont_reduction_lemma_step_modr:
   rLen:nat -> n:pos -> mu:nat -> i:pos{i <= rLen} -> c:nat -> res0:nat -> Lemma
   (requires res0 % pow2 (64 * (i - 1)) == 0 /\ (1 + n * mu) % pow2 64 == 0)
-  (ensures  smont_reduction_f rLen n mu (i - 1) res0 % pow2 (64 * i) == 0)
+  (ensures  mont_reduction_f rLen n mu (i - 1) res0 % pow2 (64 * i) == 0)
 
 let mont_reduction_lemma_step_modr rLen n mu i c res0 =
-  let res = smont_reduction_f rLen n mu (i - 1) res0 in
-  let c_i = res0 / pow2 (64 * (i - 1)) % pow2 64 in
+  let b = pow2 (64 * i) in
+  let b1 = pow2 (64 * (i - 1)) in
+
+  let res = mont_reduction_f rLen n mu (i - 1) res0 in
+  let c_i = res0 / b1 % pow2 64 in
   let q_i = mu * c_i % pow2 64 in
-  assert (res == res0 + n * q_i * pow2 (64 * (i - 1)));
+  assert (res == res0 + n * q_i * b1);
   calc (==) {
-    res % pow2 (64 * i);
+    res % b;
     (==) { }
-    (res0 + n * q_i * pow2 (64 * (i - 1))) % pow2 (64 * i);
-    (==) { Math.Lemmas.euclidean_division_definition res0 (pow2 (64 * (i -1))) }
-    (res0 / pow2 (64 * (i - 1)) * pow2 (64 * (i - 1)) + n * q_i * pow2 (64 * (i - 1))) % pow2 (64 * i);
-    (==) { Math.Lemmas.lemma_mod_plus_distr_l (res0 / pow2 (64 * (i -1)) * pow2 (64 * (i -1))) (n * q_i * pow2 (64 * (i - 1))) (pow2 (64 * i)) }
-    (res0 / pow2 (64 * (i - 1)) * pow2 (64 * (i - 1)) % pow2 (64 * i) + n * q_i * pow2 (64 * (i - 1))) % pow2 (64 * i);
-    (==) { Math.Lemmas.pow2_multiplication_modulo_lemma_2 (res0 / pow2 (64 * (i -1))) (64 * i) (64 * (i - 1)) }
-    (res0 / pow2 (64 * (i - 1)) % pow2 64 * pow2 (64 * (i - 1)) + n * q_i * pow2 (64 * (i - 1))) % pow2 (64 * i);
-    (==) { Math.Lemmas.distributivity_add_left (res0 / pow2 (64 * (i - 1)) % pow2 64) (n * q_i) (pow2 (64 * (i - 1))) }
-    (res0 / pow2 (64 * (i - 1)) % pow2 64 + n * q_i) * pow2 (64 * (i - 1)) % pow2 (64 * i);
-    (==) { Math.Lemmas.pow2_multiplication_modulo_lemma_2 (res0 / pow2 (64 * (i - 1)) % pow2 64 + n * q_i) (64 * i) (64 * (i - 1)) }
-    (res0 / pow2 (64 * (i - 1)) % pow2 64 + n * q_i) % pow2 64 * pow2 (64 * (i - 1));
+    (res0 + n * q_i * b1) % b;
+    (==) { Math.Lemmas.euclidean_division_definition res0 b1 }
+    (res0 / b1 * b1 + n * q_i * b1) % b;
+    (==) { Math.Lemmas.lemma_mod_plus_distr_l (res0 / b1 * b1) (n * q_i * b1) b }
+    (res0 / b1 * b1 % b + n * q_i * b1) % b;
+    (==) { Math.Lemmas.pow2_multiplication_modulo_lemma_2 (res0 / b1) (64 * i) (64 * (i - 1)) }
+    (res0 / b1 % pow2 64 * b1 + n * q_i * b1) % b;
+    (==) { Math.Lemmas.distributivity_add_left (res0 / b1 % pow2 64) (n * q_i) b1 }
+    (res0 / b1 % pow2 64 + n * q_i) * b1 % b;
+    (==) { Math.Lemmas.pow2_multiplication_modulo_lemma_2 (res0 / b1 % pow2 64 + n * q_i) (64 * i) (64 * (i - 1)) }
+    (res0 / b1 % pow2 64 + n * q_i) % pow2 64 * b1;
     (==) { }
-    (c_i + n * (mu * c_i % pow2 64)) % pow2 64 * pow2 (64 * (i - 1));
+    (c_i + n * (mu * c_i % pow2 64)) % pow2 64 * b1;
     (==) { Math.Lemmas.lemma_mod_plus_distr_r c_i (n * (mu * c_i % pow2 64)) (pow2 64) }
-    (c_i + n * (mu * c_i % pow2 64) % pow2 64) % pow2 64 * pow2 (64 * (i - 1));
+    (c_i + n * (mu * c_i % pow2 64) % pow2 64) % pow2 64 * b1;
     (==) { Math.Lemmas.lemma_mod_mul_distr_r n (mu * c_i) (pow2 64); Math.Lemmas.paren_mul_right n mu c_i }
-    (c_i + n * mu * c_i % pow2 64) % pow2 64 * pow2 (64 * (i - 1));
+    (c_i + n * mu * c_i % pow2 64) % pow2 64 * b1;
     (==) { Math.Lemmas.lemma_mod_plus_distr_r c_i (n * mu * c_i) (pow2 64) }
-    (c_i + n * mu * c_i) % pow2 64 * pow2 (64 * (i - 1));
+    (c_i + n * mu * c_i) % pow2 64 * b1;
     (==) { Math.Lemmas.distributivity_add_left 1 (n * mu) c_i }
-    ((1 + n * mu) * c_i) % pow2 64 * pow2 (64 * (i - 1));
+    ((1 + n * mu) * c_i) % pow2 64 * b1;
     (==) { Math.Lemmas.lemma_mod_mul_distr_l (1 + n * mu) c_i (pow2 64) }
-    ((1 + n * mu) % pow2 64 * c_i) % pow2 64 * pow2 (64 * (i - 1));
+    ((1 + n * mu) % pow2 64 * c_i) % pow2 64 * b1;
     (==) { assert ((1 + n * mu) % pow2 64 == 0) }
     0;
   };
-  assert (res % pow2 (64 * i) == 0)
+  assert (res % b == 0)
 
 
 val mont_reduction_lemma_step_modn:
   rLen:nat -> n:pos -> mu:nat -> i:pos{i <= rLen} -> c:nat -> res0:nat -> Lemma
   (requires res0 % n == c % n)
-  (ensures  smont_reduction_f rLen n mu (i - 1) res0 % n == c % n)
+  (ensures  mont_reduction_f rLen n mu (i - 1) res0 % n == c % n)
 
 let mont_reduction_lemma_step_modn rLen n mu i c res0 =
-  let res = smont_reduction_f rLen n mu (i - 1) res0 in
+  let res = mont_reduction_f rLen n mu (i - 1) res0 in
   let c_i = res0 / pow2 (64 * (i - 1)) % pow2 64 in
   let q_i = mu * c_i % pow2 64 in
   assert (res == res0 + n * q_i * pow2 (64 * (i - 1)));
@@ -299,7 +318,7 @@ val mont_reduction_lemma_step:
   (requires
     res0 % n == c % n /\ res0 % pow2 (64 * (i - 1)) == 0 /\
     res0 <= c + (pow2 (64 * (i - 1)) - 1) * n /\ (1 + n * mu) % pow2 64 == 0)
-  (ensures  (let res = smont_reduction_f rLen n mu (i - 1) res0 in
+  (ensures  (let res = mont_reduction_f rLen n mu (i - 1) res0 in
     res % n == c % n /\ res % pow2 (64 * i) == 0 /\ res <= c + (pow2 (64 * i) - 1) * n))
 
 let mont_reduction_lemma_step rLen n mu i c res0 =
@@ -310,27 +329,84 @@ let mont_reduction_lemma_step rLen n mu i c res0 =
 
 val mont_reduction_loop_lemma: rLen:nat -> n:pos -> mu:nat -> i:nat{i <= rLen} -> c:nat -> Lemma
   (requires (1 + n * mu) % pow2 64 == 0)
-  (ensures  (let res = repeati i (smont_reduction_f rLen n mu) c in
+  (ensures  (let res = repeati i (mont_reduction_f rLen n mu) c in
     res % n == c % n /\ res % pow2 (64 * i) == 0 /\ res <= c + (pow2 (64 * i) - 1) * n))
 
 let rec mont_reduction_loop_lemma rLen n mu i c =
-  let res : nat = repeati i (smont_reduction_f rLen n mu) c in
+  let res : nat = repeati i (mont_reduction_f rLen n mu) c in
   if i = 0 then
-    eq_repeati0 i (smont_reduction_f rLen n mu) c
+    eq_repeati0 i (mont_reduction_f rLen n mu) c
   else begin
-    unfold_repeati i (smont_reduction_f rLen n mu) c (i - 1);
-    let res0 : nat = repeati (i - 1) (smont_reduction_f rLen n mu) c in
+    unfold_repeati i (mont_reduction_f rLen n mu) c (i - 1);
+    let res0 : nat = repeati (i - 1) (mont_reduction_f rLen n mu) c in
     mont_reduction_loop_lemma rLen n mu (i - 1) c;
     mont_reduction_lemma_step rLen n mu i c res0 end
 
 
+val lemma_fits_aux: c:nat -> r:pos -> n:pos -> Lemma
+  (requires c < n * n /\ n < r)
+  (ensures (c - n) / r < n)
+
+let lemma_fits_aux c r n =
+  assert (c < r * n);
+  assert (c / r < n);
+  Math.Lemmas.lemma_div_le (c - n) c r
+
+
+val mont_mult_lemma_fits_aux: rLen:nat -> n:pos -> d:int -> mu:nat -> c:nat -> Lemma
+  (requires
+    (1 + n * mu) % pow2 64 == 0 /\ pow2 (64 * rLen) * d % n == 1 /\
+     n < pow2 (64 * rLen) /\ c < n * n)
+  (ensures
+    (let res : nat = repeati rLen (mont_reduction_f rLen n mu) c in
+     res / pow2 (64 * rLen) < 2 * n))
+
+let mont_mult_lemma_fits_aux rLen n d mu c =
+  let r = pow2 (64 * rLen) in
+  let res : nat = repeati rLen (mont_reduction_f rLen n mu) c in
+  mont_reduction_loop_lemma rLen n mu rLen c;
+  assert (res <= c + (r - 1) * n /\ res % r == 0);
+  Math.Lemmas.lemma_div_le res (c + (r - 1) * n) r;
+  assert (res / r <= (c + (r - 1) * n) / r);
+  calc (<) {
+    (c + (r - 1) * n) / r;
+    (==) { Math.Lemmas.distributivity_sub_left r 1 n }
+    (c - n + r * n) / r;
+    (==) { Math.Lemmas.lemma_div_plus (c - n) n r }
+    (c - n) / r + n;
+    (<) { lemma_fits_aux c r n }
+    n + n;
+  };
+  assert (res / r < 2 * n)
+
+
+val mont_mult_lemma_fits: rLen:nat -> n:pos -> d:int -> mu:nat -> c:nat -> Lemma
+  (requires
+    (1 + n * mu) % pow2 64 == 0 /\ pow2 (64 * rLen) * d % n == 1 /\
+     n < pow2 (64 * rLen) /\ c < n * n)
+  (ensures mont_reduction rLen n mu c < n)
+
+let mont_mult_lemma_fits rLen n d mu c =
+  let r = pow2 (64 * rLen) in
+  let res : nat = repeati rLen (mont_reduction_f rLen n mu) c in
+  let res = res / r in
+  mont_mult_lemma_fits_aux rLen n d mu c;
+  let res1 = if res < n then res else res - n in
+  assert (res1 < n)
+
+
 val mont_reduction_lemma: rLen:nat -> n:pos -> d:int-> mu:nat -> c:nat -> Lemma
-  (requires (1 + n * mu) % pow2 64 == 0 /\ pow2 (64 * rLen) * d % n == 1)
-  (ensures  mont_reduction rLen n mu c % n == c * d % n)
+  (requires
+    (1 + n * mu) % pow2 64 == 0 /\ pow2 (64 * rLen) * d % n == 1 /\
+    n < pow2 (64 * rLen) /\ c < n * n)
+  (ensures  mont_reduction rLen n mu c == c * d % n)
 
 let mont_reduction_lemma rLen n d mu c =
   let r = pow2 (64 * rLen) in
-  let res : nat = repeati rLen (smont_reduction_f rLen n mu) c in
+  let res : nat = repeati rLen (mont_reduction_f rLen n mu) c in
+
+  let r = pow2 (64 * rLen) in
+  let res : nat = repeati rLen (mont_reduction_f rLen n mu) c in
   mont_reduction_loop_lemma rLen n mu rLen c;
   assert (res % n == c % n /\ res % r == 0 /\ res <= c + (r - 1) * n);
   calc (==) {
@@ -350,11 +426,17 @@ let mont_reduction_lemma rLen n d mu c =
     (==) { Math.Lemmas.lemma_mod_mul_distr_l c d n }
     c * d % n;
   };
-  assert (res / r % n == c * d % n)
+  assert (res / r % n == c * d % n);
 
+  let res1 = res / r in
+  let res2 = if res1 < n then res1 else res1 - n in
+  Math.Lemmas.lemma_mod_sub res1 n 1;
+  assert (res2 % n == res1 % n);
+  mont_mult_lemma_fits rLen n d mu c;
+  Math.Lemmas.small_mod res2 n
 
 ///
-///  Lemma (to_mont rLen n mu a % n == a * pow2 (64 * rLen) % n)
+///  Lemma (to_mont rLen n mu a == a * pow2 (64 * rLen) % n)
 ///
 
 val lemma_mod_mul_distr3: a:int -> b:int -> c:int -> n:pos -> Lemma
@@ -374,8 +456,10 @@ let lemma_mod_mul_distr3 a b c n =
 
 
 val to_mont_lemma: rLen:nat -> n:pos -> d:int-> mu:nat -> a:nat -> Lemma
-  (requires (1 + n * mu) % pow2 64 == 0 /\ pow2 (64 * rLen) * d % n == 1)
-  (ensures  to_mont rLen n mu a % n == a * pow2 (64 * rLen) % n)
+  (requires
+    (1 + n * mu) % pow2 64 == 0 /\ pow2 (64 * rLen) * d % n == 1 /\
+    n < pow2 (64 * rLen) /\ a < n)
+  (ensures  to_mont rLen n mu a == a * pow2 (64 * rLen) % n)
 
 let to_mont_lemma rLen n d mu a =
   let r = pow2 (64 * rLen) in
@@ -384,7 +468,7 @@ let to_mont_lemma rLen n d mu a =
   let aM = to_mont rLen n mu a in
   assert (aM == mont_reduction rLen n mu c);
   mont_reduction_lemma rLen n d mu c;
-  assert (aM % n == c * d % n);
+  assert (aM == c * d % n);
   calc (==) {
     c * d % n;
     (==) { }
@@ -402,170 +486,17 @@ let to_mont_lemma rLen n d mu a =
     (==) { assert (r * d % n == 1) }
     a * r % n;
     };
-  assert (aM % n == a * r % n)
+  assert (aM == a * r % n)
 
 ///
-///  Lemma (from_mont rLen n mu aM % n == aM * d % n)
+///  Lemma (from_mont rLen n mu aM == aM * d % n)
 ///
 
 val from_mont_lemma: rLen:nat -> n:pos -> d:int -> mu:nat -> aM:nat -> Lemma
-  (requires (1 + n * mu) % pow2 64 == 0 /\ pow2 (64 * rLen) * d % n == 1)
-  (ensures  from_mont rLen n mu aM % n == aM * d % n)
+  (requires
+    (1 + n * mu) % pow2 64 == 0 /\ pow2 (64 * rLen) * d % n == 1 /\
+    n < pow2 (64 * rLen) /\ aM < n)
+  (ensures  from_mont rLen n mu aM == aM * d % n)
 
 let from_mont_lemma rLen n d mu aM =
   mont_reduction_lemma rLen n d mu aM
-
-
-///
-///  Fits-related lemmas
-///
-
-(* To avoid the conditional subtraction, we need to select R s.t. 4 * N < R *)
-(* It means that the montgomery multiplication will take 0 <= A, B < 2 * N and
-   return C % N = A * B * R % N /\ C < 2 * N *)
-
-val mont_preconditions_rLen: nLen:nat -> n:pos{n < pow2 (64 * nLen)} ->
-  Lemma (4 * n < pow2 (64 * (nLen + 1)))
-
-let mont_preconditions_rLen nLen n =
-  calc (<) {
-    4 * n;
-    (<) { Math.Lemmas.lemma_mult_lt_left 4 n (pow2 (64 * nLen)) }
-    4 * pow2 (64 * nLen);
-    (==) { assert_norm (pow2 2 = 4) }
-    pow2 2 * pow2 (64 * nLen);
-    (==) { Math.Lemmas.pow2_plus 2 (64 * nLen) }
-    pow2 (2 + 64 * nLen);
-    (<) { Math.Lemmas.pow2_lt_compat (64 + 64 * nLen) (2 + 64 * nLen) }
-    pow2 (64 + 64 * nLen);
-    (==) { Math.Lemmas.distributivity_add_right 64 1 nLen }
-    pow2 (64 * (nLen + 1));
-  };
-  assert (4 * n < pow2 (64 * (nLen + 1)))
-
-
-val mont_preconditions:
-  nLen:nat -> n:pos{1 < n /\ n < pow2 (64 * nLen)} -> mu:nat -> Lemma
-  (requires n % 2 = 1 /\ (1 + (n % pow2 64) * mu) % pow2 64 == 0)
-  (ensures
-    (let r = pow2 (64 * (nLen + 1)) in
-     let d, _ = eea_pow2_odd (64 * (nLen + 1)) n in
-     r * d % n == 1 /\ 4 * n < r /\ (1 + n * mu) % pow2 64 == 0))
-
-let mont_preconditions nLen n mu =
-  mont_preconditions_d (nLen + 1) n;
-  mont_preconditions_n0 n mu;
-  mont_preconditions_rLen nLen n
-
-///
-///  Lemma (mont_reduction rLen n mu c < 2 * n)
-///
-
-val lemma_fits_aux: c:nat -> r:pos -> n:pos -> Lemma
-  (requires c < 4 * n * n /\ 4 * n < r)
-  (ensures (c - n) / r < n)
-
-let lemma_fits_aux c r n =
-  assert (c < r * n);
-  assert (c / r < n);
-  Math.Lemmas.lemma_div_le (c - n) c r
-
-
-val mont_mult_lemma_fits: rLen:nat -> n:pos -> d:int -> mu:nat -> c:nat -> Lemma
-  (requires
-    (1 + n * mu) % pow2 64 == 0 /\ pow2 (64 * rLen) * d % n == 1 /\
-     4 * n < pow2 (64 * rLen) /\ c < 4 * n * n)
-  (ensures mont_reduction rLen n mu c < 2 * n)
-
-let mont_mult_lemma_fits rLen n d mu c =
-  let r = pow2 (64 * rLen) in
-  let res : nat = repeati rLen (smont_reduction_f rLen n mu) c in
-  mont_reduction_loop_lemma rLen n mu rLen c;
-  assert (res <= c + (r - 1) * n /\ res % r == 0);
-  Math.Lemmas.lemma_div_le res (c + (r - 1) * n) r;
-  assert (res / r <= (c + (r - 1) * n) / r);
-  calc (<) {
-    (c + (r - 1) * n) / r;
-    (==) { Math.Lemmas.distributivity_sub_left r 1 n }
-    (c - n + r * n) / r;
-    (==) { Math.Lemmas.lemma_div_plus (c - n) n r }
-    (c - n) / r + n;
-    (<) { lemma_fits_aux c r n }
-    n + n;
-  };
-  assert (res / r < 2 * n)
-
-
-///
-///  Lemma (to_mont rLen n mu a < 2 * n)
-///
-
-val to_mont_lemma_fits: rLen:nat -> n:pos -> d:int -> mu:nat -> a:nat -> Lemma
-  (requires
-    (1 + n * mu) % pow2 64 == 0 /\ pow2 (64 * rLen) * d % n == 1 /\
-    4 * n < pow2 (64 * rLen) /\ a < n)
-  (ensures to_mont rLen n mu a < 2 * n)
-
-let to_mont_lemma_fits rLen n d mu a =
-  let r2 = pow2 (128 * rLen) % n in
-  let c = a * r2 in
-  assert (a * r2 <= n * n);
-  let aM = mont_reduction rLen n mu c in
-  assert (a * r2 < 4 * n * n);
-  mont_mult_lemma_fits rLen n d mu c
-
-
-///
-///  Lemma (from_mont rLen n mu aM <= n)
-///
-
-val lemma_fits_aux1: aM:nat -> r:pos -> n:pos -> Lemma
-  (requires aM < 2 * n /\ 4 * n < r)
-  (ensures (aM - n) / r <= 0)
-
-let lemma_fits_aux1 aM r n =
-  assert (aM - n < n);
-  Math.Lemmas.lemma_div_le (aM - n) n r;
-  Math.Lemmas.small_division_lemma_1 n r
-
-
-val from_mont_lemma_fits: rLen:nat -> n:pos -> d:int -> mu:nat -> aM:nat -> Lemma
-  (requires
-    (1 + n * mu) % pow2 64 == 0 /\ pow2 (64 * rLen) * d % n == 1 /\
-    4 * n < pow2 (64 * rLen) /\ aM < 2 * n)
-  (ensures from_mont rLen n mu aM <= n)
-
-let from_mont_lemma_fits rLen n d mu aM =
-  let r = pow2 (64 * rLen) in
-  let res : nat = repeati rLen (smont_reduction_f rLen n mu) aM in
-  mont_reduction_loop_lemma rLen n mu rLen aM;
-  assert (res <= aM + (r - 1) * n /\ res % r == 0);
-  Math.Lemmas.lemma_div_le res (aM + (r - 1) * n) r;
-  assert (res / r <= (aM + (r - 1) * n) / r);
-  calc (<=) {
-    (aM + (r - 1) * n) / r;
-    (==) { Math.Lemmas.distributivity_sub_left r 1 n }
-    (aM - n + r * n) / r;
-    (==) { Math.Lemmas.lemma_div_plus (aM - n) n r }
-    (aM - n) / r + n;
-    (<=) { lemma_fits_aux1 aM r n }
-    n;
-  };
-  assert (res / r <= n)
-
-
-///
-///  Lemma (mont_mul rLen n mu a b < 2 * n)
-///
-
-val mont_mul_lemma_fits: rLen:nat -> n:pos -> d:int -> mu:nat -> a:nat -> b:nat -> Lemma
-  (requires
-    (1 + n * mu) % pow2 64 == 0 /\ pow2 (64 * rLen) * d % n == 1 /\
-    4 * n < pow2 (64 * rLen) /\ a < 2 * n /\ b < 2 * n)
-  (ensures mont_mul rLen n mu a b < 2 * n)
-
-let mont_mul_lemma_fits rLen n d mu a b =
-  let c = a * b in
-  Math.Lemmas.lemma_mult_lt_sqr a b (2 * n);
-  assert (c < 4 * n * n);
-  mont_mult_lemma_fits rLen n d mu c
