code/rsapss/Hacl.Spec.Bignum.Montgomery.fsti
@@ -21,7 +21,7 @@ val mod_inv_u64_lemma: n0:uint64 -> Lemma
   (ensures (1 + v n0 * v (mod_inv_u64 n0)) % pow2 64 == 0)
 
 val precomp_r2_mod_n:
-    #nLen:size_pos{128 * (nLen + 1) <= max_size_t}
+    #nLen:size_pos{128 * nLen <= max_size_t}
   -> modBits:size_pos{nLen == blocks modBits 64}
   -> n:lbignum nLen ->
   lbignum nLen
@@ -29,82 +29,75 @@ val precomp_r2_mod_n:
 val precomp_r2_mod_n_lemma: #nLen:size_pos -> modBits:size_pos -> n:lbignum nLen -> Lemma
   (requires
     0 < bn_v n /\ pow2 (modBits - 1) < bn_v n /\
-    128 * (nLen + 1) <= max_size_t /\ nLen == blocks modBits 64)
-  (ensures  bn_v (precomp_r2_mod_n modBits n) == pow2 (128 * (nLen + 1)) % bn_v n)
+    128 * nLen <= max_size_t /\ nLen == blocks modBits 64)
+  (ensures  bn_v (precomp_r2_mod_n modBits n) == pow2 (128 * nLen) % bn_v n)
 
 ///
 ///  Conversion functions to/from the Montgomery domen and the Montgomery reduction
 ///
 
 val mont_reduction:
-    #nLen:size_nat
-  -> #rLen:size_nat{rLen = nLen + 1 /\ rLen + rLen <= max_size_t}
+    #nLen:size_pos{nLen + nLen <= max_size_t}
   -> n:lbignum nLen
   -> mu:uint64
-  -> c:lbignum (rLen + rLen) ->
-  lbignum rLen
+  -> c:lbignum (nLen + nLen) ->
+  lbignum nLen
 
 
 val to_mont:
-    #nLen:size_nat
-  -> #rLen:size_nat{rLen = nLen + 1 /\ rLen + rLen <= max_size_t}
+    #nLen:size_pos{nLen + nLen <= max_size_t}
   -> n:lbignum nLen
   -> mu:uint64
   -> r2:lbignum nLen
   -> a:lbignum nLen ->
-  lbignum rLen
+  lbignum nLen
 
 
 val from_mont:
-    #nLen:size_nat
-  -> #rLen:size_nat{rLen = nLen + 1 /\ rLen + rLen <= max_size_t}
+    #nLen:size_pos{nLen + nLen <= max_size_t}
   -> n:lbignum nLen
   -> mu:uint64
-  -> aM:lbignum rLen ->
+  -> aM:lbignum nLen ->
   lbignum nLen
 
 
 val mont_mul:
-    #nLen:size_nat
-  -> #rLen:size_nat{rLen = nLen + 1 /\ rLen + rLen <= max_size_t}
+    #nLen:size_pos{nLen + nLen <= max_size_t}
   -> n:lbignum nLen
   -> mu:uint64
-  -> aM:lbignum rLen
-  -> bM:lbignum rLen ->
-  lbignum rLen
+  -> aM:lbignum nLen
+  -> bM:lbignum nLen ->
+  lbignum nLen
 
 
 val mont_sqr:
-    #nLen:size_nat
-  -> #rLen:size_nat{rLen = nLen + 1 /\ rLen + rLen <= max_size_t}
+    #nLen:size_pos{nLen + nLen <= max_size_t}
   -> n:lbignum nLen
   -> mu:uint64
-  -> aM:lbignum rLen ->
-  lbignum rLen
+  -> aM:lbignum nLen ->
+  lbignum nLen
 
 ///
 ///  Lemmas
 ///
 
 val mont_reduction_lemma:
-    #nLen:size_nat
-  -> #rLen:size_nat{rLen = nLen + 1 /\ rLen + rLen <= max_size_t}
+    #nLen:size_pos{nLen + nLen <= max_size_t}
   -> n:lbignum nLen
   -> mu:uint64
-  -> c:lbignum (rLen + rLen) -> Lemma
+  -> c:lbignum (nLen + nLen) -> Lemma
   (requires
     (1 + (bn_v n % pow2 64) * v mu) % pow2 64 == 0 /\
     bn_v n % 2 = 1 /\ 1 < bn_v n /\ bn_v n < pow2 (64 * nLen) /\
-    bn_v c < 4 * bn_v n * bn_v n)
+    bn_v c < bn_v n * bn_v n)
   (ensures
-    (let res = bn_v (mont_reduction #nLen #rLen n mu c) in
-    res == M.mont_reduction rLen (bn_v n) (v mu) (bn_v c) /\
-    res < 2 * bn_v n))
+    (let res = bn_v (mont_reduction #nLen n mu c) in
+    res == M.mont_reduction nLen (bn_v n) (v mu) (bn_v c) /\
+    res < bn_v n))
 
 
 val to_mont_lemma:
-    #nLen:size_nat
-  -> #rLen:size_nat{rLen = nLen + 1 /\ rLen + rLen <= max_size_t}
+    #nLen:size_pos{nLen + nLen <= max_size_t}
   -> n:lbignum nLen
   -> mu:uint64
   -> r2:lbignum nLen
@@ -112,57 +105,54 @@ val to_mont_lemma:
   (requires
     (1 + (bn_v n % pow2 64) * v mu) % pow2 64 == 0 /\
     bn_v n % 2 = 1 /\ 1 < bn_v n /\ bn_v n < pow2 (64 * nLen) /\
-    bn_v a < bn_v n /\ bn_v r2 == pow2 (128 * rLen) % bn_v n)
+    bn_v a < bn_v n /\ bn_v r2 == pow2 (128 * nLen) % bn_v n)
   (ensures
-   (let aM = bn_v (to_mont #nLen #rLen n mu r2 a) in
-    aM == M.to_mont rLen (bn_v n) (v mu) (bn_v a) /\
-    aM < 2 * bn_v n))
+   (let aM = bn_v (to_mont #nLen n mu r2 a) in
+    aM == M.to_mont nLen (bn_v n) (v mu) (bn_v a) /\
+    aM < bn_v n))
 
 
 val from_mont_lemma:
-    #nLen:size_nat
-  -> #rLen:size_nat{rLen = nLen + 1 /\ rLen + rLen <= max_size_t}
+    #nLen:size_pos{nLen + nLen <= max_size_t}
   -> n:lbignum nLen
   -> mu:uint64
-  -> aM:lbignum rLen -> Lemma
+  -> aM:lbignum nLen -> Lemma
   (requires
     (1 + (bn_v n % pow2 64) * v mu) % pow2 64 == 0 /\
     bn_v n % 2 = 1 /\ 1 < bn_v n /\ bn_v n < pow2 (64 * nLen) /\
-    bn_v aM < 2 * bn_v n)
+    bn_v aM < bn_v n)
   (ensures
-   (let a = bn_v (from_mont #nLen #rLen n mu aM) in
-    a == M.from_mont rLen (bn_v n) (v mu) (bn_v aM) /\
-    a <= bn_v n))
+   (let a = bn_v (from_mont #nLen n mu aM) in
+    a == M.from_mont nLen (bn_v n) (v mu) (bn_v aM) /\
+    a < bn_v n))
 
 
 val mont_mul_lemma:
-    #nLen:size_nat
-  -> #rLen:size_nat{rLen = nLen + 1 /\ rLen + rLen <= max_size_t}
+    #nLen:size_pos{nLen + nLen <= max_size_t}
   -> n:lbignum nLen
   -> mu:uint64
-  -> aM:lbignum rLen
-  -> bM:lbignum rLen -> Lemma
+  -> aM:lbignum nLen
+  -> bM:lbignum nLen -> Lemma
   (requires
     (1 + (bn_v n % pow2 64) * v mu) % pow2 64 == 0 /\
     bn_v n % 2 = 1 /\ 1 < bn_v n /\ bn_v n < pow2 (64 * nLen) /\
-    bn_v aM < 2 * bn_v n /\ bn_v bM < 2 * bn_v n)
+    bn_v aM < bn_v n /\ bn_v bM < bn_v n)
   (ensures
-    (let res = bn_v (mont_mul #nLen #rLen n mu aM bM) in
-    res == M.mont_mul rLen (bn_v n) (v mu) (bn_v aM) (bn_v bM) /\
-    res < 2 * bn_v n))
+    (let res = bn_v (mont_mul #nLen n mu aM bM) in
+    res == M.mont_mul nLen (bn_v n) (v mu) (bn_v aM) (bn_v bM) /\
+    res < bn_v n))
 
 
 val mont_sqr_lemma:
-    #nLen:size_nat
-  -> #rLen:size_nat{rLen = nLen + 1 /\ rLen + rLen <= max_size_t}
+    #nLen:size_pos{nLen + nLen <= max_size_t}
   -> n:lbignum nLen
   -> mu:uint64
-  -> aM:lbignum rLen -> Lemma
+  -> aM:lbignum nLen -> Lemma
   (requires
     (1 + (bn_v n % pow2 64) * v mu) % pow2 64 == 0 /\
     bn_v n % 2 = 1 /\ 1 < bn_v n /\ bn_v n < pow2 (64 * nLen) /\
-    bn_v aM < 2 * bn_v n)
+    bn_v aM < bn_v n)
   (ensures
-    (let res = bn_v (mont_sqr #nLen #rLen n mu aM) in
-    res == M.mont_mul rLen (bn_v n) (v mu) (bn_v aM) (bn_v aM) /\
-    res < 2 * bn_v n))
+    (let res = bn_v (mont_sqr #nLen n mu aM) in
+    res == M.mont_mul nLen (bn_v n) (v mu) (bn_v aM) (bn_v aM) /\
+    res < bn_v n))
